# Quadratic Identities
## $(a+b)^2$
> $(a+b)^{2} = a^{2} + b^{2}+ ab + ba$
> 
> = $(a+b)^{2}= a^{2}+b^2+2ab$

## $(a-b)^2$
> $(a-b)^{2} = a^{2} + b^{2}- ab - ba$
> 
> = $(a+b)^{2}= a^{2} + b^{2} - 2ab$

## $a^{2} - b^{2}$
> $a^{2} - b^{2} = a(a -b) + b(a - b)$
> 
> = $(a+b)^{2}= (a+b)(a-b)$

## $(a+b+c)^2$
> $(a+b+c)^{2} = a(a + b + c) + b(a+b+c)+c(a+b+c)$
> 
> $= a^{2} + b^{2}+c^2+2ab+2bc+2ac$

# Cubic Identities
## $(x+y)^3$
> $(x+y)^{3}=(x+y)(x+y)(x+y)$
> 
> $= (x+y)[x(x+y) + y(x+y)]$
> 
> $= (x+y)(x+y)^2$
> 
> $=x(x^2+y^2+2xy)+y(x^2+y^2+2xy)$
> 
> $= x^3+xy^2+2x^2y+x^2y+y^3+2xy^2$
> 
> $=x^3+y^3+3xy^2+3x^2y$
> 
> $= x^3+y^3+3xy(x+y)$

## $(x-y)^3$
> $(x-y)^{3}=(x-y)(x-y)(x-y)$
> 
> $= (x-y)[x(x-y) - y(x-y)]$
> 
> $= (x-y)(x-y)^2$
> 
> $=x(x^2+y^2-2xy)+y(x^2+y^2-2xy)$
> 
> $= x^3+xy^2-2x^2-x^2y+y^3+2xy^2$
> 
> $=x^3+y^3+3xy^2-3x^2y$
> 
> $= x^3+y^3-3xy(x-y)$

## $x^3+y^3+z^3-3xyz$
> $x^3+y^3+z^3-3xyz=(x+y+z)(x^2+y^2+z^2-2xy-2yz-2xz)$